\documentclass[openany]{book}

\usepackage[margin=1in]{geometry}
\usepackage{amsmath,amsfonts,amsthm, amssymb}
\usepackage{yhmath}
\usepackage{mathrsfs}
\usepackage{mathtools}
\usepackage{xcolor}
\usepackage{graphicx}
\usepackage{comment}
\usepackage{tikz-cd}
\usepackage{quiver}
\renewcommand{\familydefault}{ppl}
\newcommand{\tr}{\text{tr}}
\newcommand{\R}{\mathbb{R}}
\newcommand{\E}{\mathbb{E}}
\newcommand{\Z}{\mathbb{Z}}
\newcommand{\C}{\mathbb{C}}
\newcommand{\F}{\mathbb{F}}
\newcommand{\la}{\langle}
\newcommand{\ra}{\rangle}
\newcommand{\colim}{\text{colim}}
\DeclareMathOperator{\im}{im}
\let\oldemptyset\emptyset
\let\emptyset\varnothing
\newcommand{\tor}{\text{Tor}}
\newcommand{\id}{\text{id}}
\newcommand{\ext}{\text{Ext}}
\newcommand{\ptop}{\text{PTop}}
\newcommand{\pt}{\text{pt}}
\newcommand{\ach}{\text{Ach}}
\newcommand{\Q}{\mathbb{Q}}
\newcommand{\gal}{\text{Gal}}


\input{hui.tex}

\title{Calc III Sections
\\ 
\vspace{0.4cm}
\large Fall 2025}




\date{\today}
\author{Hui Sun}


\begin{document}

\maketitle

% \tableofcontents
\newpage


\begin{center}
    \Large Calc III-Week 5 (9/22-9/26)
\end{center}

\renewcommand\thesection{\arabic{section}}

\noindent
Topics: (1) properties of derivatives, (2) directional derivatives, (3) gradient.


% (Section 2.5 on the multivariable chain rule and Section 2.6 on gradients and directional derivatives.

% I would like you to spend about 15-20 minutes going through some chain rule problems e.g. something like problems 7 or 8 from Section 2.5. One problem I really like that reviews multiple different concepts is 11 from Section 2.5 If you could present this problem, I think that would be good for the students
 
% key concept: the matrix of partial derivatives. 
 
% Please use the rest of the time to start discussing Section 2.6, specifically focusing on pg. 135-139. I will try to go through these pages on Monday, but I may have to go quickly. Reviewing all this material with simple examples is what I would recommend. Some problems that could be relevant are 3, 6, and 7 from Section 2.6).


\begin{defn}[path]
    A \textbf{path} $c$ is a map $c: [a,b]\to \R^n$. We can write $c(t)=(c_1(t), \dots, c_n(t))$. If $c$ is differentiable, then we can define the \textbf{velocity} of $c$ at any $t_0\in [a,b]$ as 
    \begin{equation*}
        c'(t_0)=\left(c_1'(t_0), \dots, c_n'(t_0)\right)
    \end{equation*}
    The velocity vector of $c$ at $t_0$ is also a \textbf{tangent} vector to $c$ at $t_0$. The \textbf{speed} of the path $c$ at $t_0$ is the length of the velocity vector $\|c'(t_0)\|$.
\end{defn}

\begin{defn}[tangent line to a path]
    Let $c:[a,b]\to\R^n$ be a path, if $c'(t_0)\neq 0$, then the \textbf{tangent line} at $x_0$ is given by 
    \begin{equation*}
        l(t)=c(t_0)+c'(t_0)(t-t_0)
    \end{equation*}
\end{defn}





\begin{prop}
    Let $f:U\subset\R^n\to\R^m$ be differentiable at $x_0$, then the derivative of $f$ at $x_0$ is an $m\times n$ matrix $Df(x_0)=\left(\frac{\partial f_i}{\partial x_j}\right)_{ij}$. The derivative follows the same properties as derivative for single variable functions:
    \begin{enumerate}
        \item Let $c\in\R$, then 
        \begin{equation*}
            D(cf)(x_0)=cDf(x_0) \tag {multiplication of a matrix by constant $c$}
        \end{equation*}
        \item Let $g: U\subset\R^n\to\R^m$ also be differentiable at $x_0$, then 
        \begin{equation*}
            D(f+g)(x_0)=Df(x_0)+Dg(x_0) \tag{sum of two matrices}
        \end{equation*}
        \item Let $h_1: U\subset\R^n\to\R, h_2: U\subset\R^n\to\R$,then 
        \begin{equation*}
            D(h_1h_2)(x_0)=Dh_1(x_0)h_2(x_0)+h_1(x_0)Dh_2(x_0) \tag{product rule}
        \end{equation*}
        and if $h_2\neq 0$ on $U$.
        \begin{equation*}
            D(h_1/h_2)(x_0)=\frac{Dh_1(x_0)h_2(x_0)-h_1(x_0)Dh_2(x_0)}{h_2^2(x_0)} \tag{quotient rule}
        \end{equation*}
        \item Let $g: U\subset\R^n\to\R^m, f:V\subset\R^m\to\R^p$ such that $g(U)\subset V$, then 
        \begin{equation*}
            D(f\circ g)(x_0)=Df(g(x_0))Dg(x_0) \tag{chain rule}
        \end{equation*}
    \end{enumerate}
\end{prop}

\begin{defn}[directiona derivative]
    Let $f:\R^3\to\R$, be differentiable, then the directional directive at $x_0\in\R^3$ in the direction of a \textbf{unit vector} $v$ is given by 
    \begin{equation*}
        \nabla f(x_0)\cdot v=\left[\frac{\partial f}{\partial x_1}(x_0)\right]v_1+\left[\frac{\partial f}{\partial x_2}(x_0)\right]v_2+\left[\frac{\partial f}{\partial x_3}(x_0)\right]v_3
    \end{equation*}
    where $v=(v_1,v_2,v_3)$.
\end{defn}

\begin{prop}
    Suppose that $\nabla f(x_0)\neq 0$, then the direction for which $f$ increases the fastest at $x_0$ is along $\nabla f(x_0)$.
\end{prop}


\begin{prop}
    Let $f:\R^3\to\R$ be differentiable, let $S$ be a level surface of $f$, i.e., $S$ is a surface described by 
    \begin{equation*}
        f(x,y,z)=k
    \end{equation*}
    were $k$ is some constant. Let $(x_0,y_0,z_0)\in S$, then
    \begin{equation*}
        \nabla f(x_0,y_0,z_0) \text{ is normal to the level surface at } (x_0,y_0,z_0)
    \end{equation*}
    This means if $c(t)$ is a path in $S$, and $v(0)=(x_0,y_0,z_0)$, and if $v$ is a tangent vector to $c(t)$ at $t=0$, then 
    \begin{equation*}
        \nabla f(x_0,y_0, z_0)\cdot v=0
    \end{equation*}
    Moreover, if $\nabla f(x_0,y_0,z_0)\neq 0$, the \textbf{tangent plane} of $S$ at $(x_0,y_0,z_0)$ is given by 
    \begin{equation*}
        \nabla f(x_0,y_0,z_0)\cdot (x-x_0, y-y_0, z-z_0)=0
    \end{equation*}
\end{prop}










\begin{prob}
    Consider the curve in $\R$: $c(t)=(2t, t^2,-t)$. Find the speed of the $c$ at $t=2$ and the tangent line at $t=1$.
\end{prob}
% \begin{proof}
%     The velocity vector of $c$ at $t=2$ is 
%     \begin{equation*}
%         c'(t)=(2, 2t, -1)
%     \end{equation*}
%     evaluated at $t=2$ is $c'(2)=(2, 4, -1)$. Thus the speed is the length of the velocity vector 
%     \begin{equation*}
%         \|c'(2)\|=\left(2^2+4^2+(-1)^2\right)^\frac{1}{2}=\sqrt{21}
%     \end{equation*}
%     For the tangent line: the tangent vector is 
%     \begin{equation*}
%         c'(1)=(2,2, -1)
%     \end{equation*}
%     and $c(1)=(2, 1, -1)$. Thus the tangent line $l$ at $t=1$ is given by 
%     \begin{equation*}
%         l(t)=(2,1,-1)+t(2,2,-1)=(2+2t, 1+2t, -1-t)
%     \end{equation*}
% \end{proof}



\begin{prob}[2.5, Q7]
    Let \( f(u, v) = (\tan (u - 1) - e^v, u^2 - v^2) \) and  
   \[
   g(x, y) = (e^{x-y}, x - y).
   \]  
   Calculate \( f \circ g \) and  
   \[
   D(f \circ g)(1, 1).
   \]
\end{prob}
% \begin{proof}
%     We have 
%     \begin{equation*}
%         f\circ g(x,y)=(\tan(e^{x-y}-1)-e^{x-y}, e^{2(x-y)}-(x-y)^2)
%     \end{equation*}
%     and $g(1,1)=(1,0)$, thus using chain rule, we have 
%     \begin{equation*}
%         D(f\circ g)(1,1)=Df(1,0)Dg(1,1)
%     \end{equation*}
%     where 
%     \begin{equation*}
%         Df(u,v)=\begin{bmatrix}
%             \sec^2(u-1)& -e^v\\
%             2u&-2v
%         \end{bmatrix}, \quad Dg(x,y)=\begin{bmatrix}
%             e^{x-y}&-e^{x-y}\\
%             1&-1
%         \end{bmatrix}
%     \end{equation*}
%     Hence 
%     \begin{align*}
%         D(f\circ g)(1,1)&=\begin{bmatrix}
%             1&-1\\
%             2&0
%         \end{bmatrix}\begin{bmatrix}
%             1&-1\\
%             1&-1
%         \end{bmatrix}\\
%         &=\begin{bmatrix}
%             0&0\\
%             2&-2
%         \end{bmatrix}
%     \end{align*}
% \end{proof}

\begin{prob}[2.5, Q8]
    Let \( f(u, v, w) = (e^{u-w}, \cos (v + u) + \sin (u + v + w)) \) and \( g(x, y) = (e^x, \cos (y - x), e^{-y}). \)  
   Calculate \( f \circ g \) and \( D(f \circ g)(0, 0)\).
\end{prob}
% \begin{proof}
%     We have 
%     \begin{equation*}
%         f\circ g =(e^{e^x-\cos(y-x)}, \cos(e^x+\cos(y-x)), \sin(e^{x}+e^{-y}+\cos(y-x)))
%     \end{equation*}
%     and $g(0,0)=(1, 1, 1)$. Thus 
%     \begin{equation*}
%         D(f\circ g)(0,0)=Df(1,1,1)Dg(0,0)
%     \end{equation*}
%     where 
%     \begin{equation*}
%         Df(u,v,w)=\begin{bmatrix}
%             e^{u-w}&0&-e^{u-w}\\
%             -\sin(v+u)+\cos(u+v+w)&-\sin(v+u)+\cos(u+v+w)&\cos(u+v+w)
%         \end{bmatrix}
%     \end{equation*}
%     and 
%     \begin{equation*}
%         Dg(x,y)=\begin{bmatrix}
%             e^x&0\\
%             \sin(y-x)&-\sin(y-x)\\
%             0&-e^{-y}
%         \end{bmatrix}
%     \end{equation*}
%     Thus 
%     \begin{align*}
%         D(f\circ g)(0,0)&=\begin{bmatrix}
%             1&0&-1\\
%             -\sin 2+\cos 3&-\sin 2+\cos 3&\cos 3
%         \end{bmatrix}\begin{bmatrix}
%             1&0\\
%             0&0\\
%             0&-1
%         \end{bmatrix}\\
%         &=\begin{bmatrix}
%             1&1\\
%             -\sin 2+\cos 3&-\cos 3
%         \end{bmatrix}
%     \end{align*}
% \end{proof}

\begin{prob}[2.5, Q11]
Let \( f(x, y, z) = (3y + 2, x^2 + y^2, x + z^2) \). Let  
\[
c(t) = (\cos(t), \sin(t), t).
\]  

(a) Find the path \( p = f \circ c \) and the velocity vector  
\[
p'(\pi).
\]  

(b) Find \( c(\pi), c'(\pi) \) and \( Df(-1, 0, \pi). \)  

(c) Thinking of \( Df(-1, 0, \pi) \) as a linear map, find  
\[
Df(-1, 0, \pi) \ (c'(\pi)).
\]
\end{prob}
% \begin{proof}
%     \begin{enumerate}
%         \item[(a)] We have 
%         \begin{equation*}
%             p(t)=(3\sin t+2, 1, \cos t+t^2)
%         \end{equation*}
%         and 
%         \begin{equation*}
%             p'(t)=(3\cos t+0, -\sin t+2t)
%         \end{equation*}
%         thus 
%         \begin{equation*}
%             p'(\pi)=(-3,0,2\pi)
%         \end{equation*}
%         \item[(b)] We have $c(\pi)=(-1, 0, \pi)$, and $c'(t)=(-\sin t, \cos t, 1)$, and $c'(\pi)=(0,-1, 1)$. And 
%         \begin{equation*}
%             Df(x,y,z)=\begin{bmatrix}
%                 0&3&0\\
%                 2x&2y&0\\
%                 1&0&2z
%             \end{bmatrix}
%         \end{equation*}
%         Thus 
%         \begin{equation*}
%             Df(-1,0,\pi)=\begin{bmatrix}
%                 0&3&0\\
%                 -2&0&0\\
%                 1&0&2\pi
%             \end{bmatrix}
%         \end{equation*}
%         \item[(c)] We have 
%         \begin{equation*}
%             Df(-1,0,\pi)(c'(\pi))=\begin{bmatrix}
%                 0&3&0\\
%                 -2&0&0\\
%                 1&0&2\pi
%             \end{bmatrix}\begin{bmatrix}
%                 0\\
%                 -1\\
%                 1
%             \end{bmatrix}=\begin{bmatrix}
%                 -3\\
%                 0\\
%                 2\pi
%             \end{bmatrix}
%         \end{equation*}
%     \end{enumerate}
% \end{proof}


\begin{prob}[2.6, Q3]
Compute the directional derivatives of the following functions along unit vectors at the indicated points in directions parallel to the given vector:

% (a) \[ f(x, y) = x^y , \((x_0, y_0) = (e, e)\), \mathbf{d} = 5\mathbf{i} + 12\mathbf{j} \]
(a)
\begin{equation*}
    f(x, y) = x^y, (x_0, y_0) = (e, e), \quad \mathbf{d} = 5\mathbf{i} + 12\mathbf{j}
\end{equation*}

(b)  
\[
f(x, y, z) = e^x + yz, \, (x_0, y_0, z_0) = (1, 1, 1), \quad \mathbf{d} = (1, -1, 1)
\]

(c)  
\[
f(x, y, z) = xyz, \, (x_0, y_0, z_0) = (1, 0, 1), \quad \mathbf{d} = (1, 0, -1)
\]
\end{prob}
% \begin{proof}
%     We find $\nabla f$ for all these functions and find the directional directive 
%     \begin{equation*}
%         \nabla f(x_0)\cdot \frac{d}{\|d\|}
%     \end{equation*}
%     \begin{enumerate}
%         \item[(a)] We have 
%         \begin{equation*}
%             \nabla f(x,y,z)=(yx^{y-1}, x^y\ln x)
%         \end{equation*}
%         hence 
%         \begin{equation*}
%             \nabla f(e,e)\cdot \frac{d}{\|d\|}=(e^e,e^e)\cdot\left(\frac{5}{13},\frac{12}{13}\right)=\frac{17}{13}e^e
%         \end{equation*}
%         \item[(b)] We have 
%         \begin{equation*}
%             \nabla f(x,y,z)=(e^x, z, y)
%         \end{equation*}
%         hence 
%         \begin{equation*}
%             \nabla f(1,1,1)\cdot \frac{1}{\sqrt{3}}(1,-1,1)=\frac{e}{\sqrt{3}}
%         \end{equation*}
%         \item[(c)] We have 
%         \begin{equation*}
%             \nabla f(x,y,z)=(yz, xz, xy)
%         \end{equation*}
%         hence 
%         \begin{equation*}
%             \nabla f(1,0,1)\cdot \frac{1}{\sqrt{2}}(1,0,-1)=\frac{1}{\sqrt{2}}(0,1,0)\cdot(1,0,-1)=0
%         \end{equation*}
%     \end{enumerate}
% \end{proof}

\begin{prob}[2.6, Q6]
Find a vector which is normal to the curve  
\[
x^3 + xy + y^3 = 11 \text{ at } (1, 2).
\]
\end{prob}
% \begin{proof}
%     Consider the function $f(x,y)=x^3+xy+y^3$, then the level set of $f(x,y)=11$ coincides with the curve above. Thus it suffices to compute 
%     \begin{equation*}
%         \nabla f(x,y)=(3x^2+y, x+3y^2)
%     \end{equation*}
%     and 
%     \begin{equation*}
%         \nabla f(1,2)=(5, 13)
%     \end{equation*}
%     is perpendicular to the the level curve.
% \end{proof}



\begin{prob}[2.6, Q7]
Find the rate of change of \( f(x, y, z) = xyz \) in the direction normal to the surface  
\[
yx^2 + xy^2 + yz^2 = 3 \text{ at } (1, 1, 1).
\]
\end{prob}

\noindent 
\textbf{Summary}
\begin{itemize}
    \item If asked to find directional derivative/rate of change along a unit vector $v$ at point $x_0$: find $\nabla f(x_0)\cdot v$.
    \item If asked to find along with direction $f$ increases the fastest: find $\nabla f(x_0)$.
    \item 
\end{itemize}



% \begin{proof}
%     We first find a normal vector to the surface, consider the surface as a level set of the function 
%     \begin{equation*}
%         g(x,y,z)=yx^2+xy^2+yz^2
%     \end{equation*}
%     Thus 
%     \begin{equation*}
%         \nabla g(x,y,z)=(2xy+y^2, x^2+2xy+z^2, 2yz)
%     \end{equation*}
%     hence 
%     \begin{equation*}
%         u=\nabla g(1,1,1)=(3, 4, 2)
%     \end{equation*}
%     is a normal vector to the surface, and we normalize it to get a unit normal vector $n=\frac{u}{\|u\|}=\frac{1}{\sqrt{29}}(3,4,2)$. Now we find the directional derivative of $f(x,y,z)=xyz$ along $(3,4,2)$:
%     \begin{equation*}
%         \nabla f(x,y,z)=(yz, xz, xy)
%     \end{equation*}
%     hence 
%     \begin{equation*}
%         \nabla f(1,1,1)=(1,1,1)
%     \end{equation*}
%     and the directional derivative is 
%     \begin{equation*}
%         \nabla f(1,1,1)\cdot n=\frac{9}{\sqrt{29}}
%     \end{equation*}
% \end{proof}





 


























\end{document}